\input ../auxiliar
\titulo{Ejercicio 19.13}

\enunciado{A continuaci\'on se muestra otra ecuaci\'on s\'olo para
practicar:}

$$\eqalignno{
\left(\int_{-\infty}^{\infty}\!e^{-x^2}\,dx\right)^2&=
\int_{-\infty}^{\infty}\int_{-\infty}^{\infty}\!e^{-(x^2+y^2)}\,dx\,dy\cr
&=\int_{0}^{2\pi}\int_{-\infty}^{\infty}\!e^{-r^2}r\,dr\,d\theta\cr
&=\int_{0}^{2\pi}\left(-{e^{-r^2}\over2}\bigg\vert_{r=0}^{r=\infty}\right)\,d\theta\cr
&=\pi.&(11)\cr
}$$

\bigskip

\respuestaS

\noindent|$$\eqalignno{|

\noindent|\left(\int_{-\infty}^{\infty}\!e^{-x^2}\,dx\right)^2&=|

\noindent|\int_{-\infty}^{\infty}\int_{-\infty}^{\infty}\!e^{-(x^2+y^2)}\,dx\,dy\cr|

\noindent|&=\int_{0}^{2\pi}\int_{-\infty}^{\infty}\!e^{-r^2}r\,dr\,d\theta\cr|

\noindent|&=\int_{0}^{2\pi}\left(-{e^{-r^2}\over2}\bigg\vert_{r=0}^{r=\infty}\right)\,d\theta\cr|

\noindent|&=\pi.&(11)\cr|

\noindent|}$$|

\bye

